iris/ProofKforkMain.v
@@ -495,7 +495,7 @@ Section KforkArms.
          (SpecAllocproc.forkret_pc :: add_vec ks (mword_of_int 4096) :: rest)) -∗
     IntrDefs.arm_pay KT1 lvl eb pme -∗
     kalloc_env_at fsc_kalloc fsc_kpages None -∗
-    is_lock γw wait_lock_addr "wait_lock"%string <{ wait_res }> -∗
+    is_lock γw wait_lock_addr "wait_lock"%string wait_res_at -∗
     is_ftable γl γf -∗
     is_itable2 fsc_itlock fsc_ic fsc_fs fsc_ireg fsc_cov fsc_logst icfg_nib icfg_dev -∗
     itable_inv -∗
