iris/SpecKfork.v
@@ -240,8 +240,8 @@ Definition wp_kfork_sconf_body
   cpu_own lvl eb pme b lks -∗
   kernel_text -∗ pc_is pcE -∗
   procs_inv γs -∗
-  is_lock γp alp_pid_lock "nextpid"%string <{ nextpid_res }> -∗
-  is_lock γw wait_lock_addr "wait_lock"%string <{ wait_res }> -∗
+  is_lock γp alp_pid_lock "nextpid"%string nextpid_res_at -∗
+  is_lock γw wait_lock_addr "wait_lock"%string wait_res_at -∗
   is_ftable γl γf -∗
   is_itable2 fsc_itlock fsc_ic fsc_fs fsc_ireg fsc_cov fsc_logst icfg_nib icfg_dev -∗
   itable_inv -∗
